---
title: "Differentiation and Integration - Lesson 3 - Example 1"
disableToc: true
math: true
---

### [Dashboard]() --> [Differentiation and Integration](Differentiation%20and%20Integration/Differentiation%20and%20Integration.md) --> [Lesson 3](Differentiation%20and%20Integration/Lesson%203.md)

$f(x) = \frac{\class{salmon}{2x + 3}}{\class{blue}{x^{2}+ 1}}$<br>
$f(x) = \frac{\htmlClass{salmon}{t(x)}}{\htmlClass{blue}{n(x)}}$<br>
<br>
**With:**<br>
$t(x) = \class{salmon}{2x + 3}$<br>
$n(x) = \class{blue}{x^{2} + 1}$<br>
<br>
**Solution:**<br>
$t'(x) = 2$<br>
$n'(x) = 2x$<br>
$f'(x) = \frac{\htmlClass{blue}{n(x)}\cdot\htmlClass{salmon}{t'(x)} - \htmlClass{salmon}{t(x)}\cdot\htmlClass{blue}{n'(x)}}{\htmlClass{blue}{n(x)}^2} = \frac{(\htmlClass{blue}{x^{2}+ 1})\cdot \htmlClass{salmon}{2} - (\htmlClass{salmon}{2x + 3})\cdot(\htmlClass{blue}{2x})}{(\htmlClass{blue}{x^{2}+ 1})^{2}}= \frac{-2x^{2}- 6x+2}{(x^{2} + 1)^{2}}$<br>
