---
title: "Differentiation and Integration - Lesson 2"
disableToc: true
math: true
---

### [Dashboard]() --> [Differentiation and Integration](Differentiation%20and%20Integration/Differentiation%20and%20Integration.md)

# <span class="highlight-blue">The sum rule</span>
The <span class="blue">derivative</span> of the <span class="blue">sum of two functions</span> is the <span class="blue">sum of the derivative</span> of the two funtions.
$$f(x) = g(x) + h(x)$$
$$f'(x) = g'(x) + h'(x)$$
<br>
[Example](Differentiation%20and%20Integration/Lesson%202%20-%20Example%201.md)
<br>

# <span class="highlight-blue">The product rule</span>
$$f(x) = g(x) \cdot h(x)$$
$$f'(x) = g'(x)\cdot h(x) + g(x)\cdot h'(x)$$
<br>
[Example](Differentiation%20and%20Integration/Lesson%202%20-%20Example%202.md)<br>
<br>

## <span class="highlight-seagreen">Invert</span>
$$f(x) = \frac{1}{x} = x^{-1}$$
$$f'(x) = -x^{-2}=-\frac{1}{x^{2}}$$
<br>

## <span class="highlight-seagreen">Powers</span>
$$f(x) = x^n$$
$$f'(x) = n\cdot x^{n - 1}$$
<br>

## <span class="highlight-seagreen">Root</span>
$$f(x) = \sqrt{x} = x^{\frac{1}{2}}$$
$$f'(x) = \frac{1}{2}x^{\frac{-1}{2}}=\frac{1}{2\sqrt{x}}$$
<br>

# <span class="highlight-fushia">Sum up</span>
<span class="fushia">Constant multiplication</span>: $[c\cdot f']=c\cdot f'$<br>
<span class="fushia">Sum</span>: $[f + g]' = f' + g'$<br>
<span class="fushia">Product</span>: $[f\cdot g]' = f'\cdot g + f\cdot g'$

|     f(x)      |         f'(x)         |
|:-------------:|:---------------------:|
|      $c$      |          $0$          |
|      $x$      |          $1$          |
|    $x^{n}$    |  $n\cdot x^{n - 1}$   |
|  $\sqrt{x}$   | $\frac{1}{2\sqrt{x}}$ |
| $\frac{1}{x}$ |  $-\frac{1}{x^{2}}$   | 
|   $\sin(x)$   |       $\cos(x)$       |
|   $\cos(x)$   |      $-\sin(x)$       |

